thys/nrest/NREST_Main.thy
@@ -544,4 +544,34 @@ shows "bindT m f \<le>  \<Down> R (\<Down>\<^sub>C E (bindT m' f'))"
   by (auto dest: inres_if_inresT_acost)
 
 
+
+
+
+definition "project_all T =  (Sum_any (the_enat o the_acost T))"
+
+lemma  project_all_is_Sumany_if_lifted:
+  "f = lift_acost g \<Longrightarrow> project_all f = (Sum_any (the_acost g))"
+  unfolding project_all_def lift_acost_def
+  by simp
+
+
+definition "norm_cost_tag a b = (a=b)"
+
+lemma norm_cost_tagI: "norm_cost_tag a a"
+  unfolding norm_cost_tag_def
+  by simp
+
+
+lemma the_acost_mult_eq_z_iff: "the_acost (n *m c) a = 0 \<longleftrightarrow> the_acost c a = 0 \<or> n=0" for n :: nat 
+  apply (cases c)
+  apply (auto simp: costmult_def)
+  done
+  
+lemma finite_the_acost_mult_nonzeroI: "finite {a. the_acost c a \<noteq> 0} \<Longrightarrow> finite {a. the_acost (n *m c) a \<noteq> 0}" for n :: nat 
+  apply (erule finite_subset[rotated])
+  by (auto simp: the_acost_mult_eq_z_iff)
+  
+  
+
+
 end
